src/proof/controllers/statefulset/progress.v
@@ -1,4 +1,4 @@
-From New.proof.controllers.statefulset Require Export pod.
+From New.proof.controllers.statefulset Require Export distance.
 
 Section proof.
 Context `{hG: !heapGS Σ} `{!ffi_semantics _ _}.
@@ -39,206 +39,31 @@ Defined.
 Context `{!kubernetesModelG Σ}.
 Local Set Default Proof Using "All".
 
-Definition missing_pod_keys sts (pods : list PodV.t) : list KKey.t :=
-  filter (λ key, key ∉ (PodV.key <$> pods)) (desired_pod_keys sts).
-
-Definition needed_pods sts pods : list PodV.t :=
-  filter (λ pod, pod_key_is_desired sts (PodV.key pod)) pods.
-
-Definition outdated_pods sts pods : list PodV.t :=
-  filter (λ pod, ¬ pod_match sts pod) (needed_pods sts pods).
-
-Definition bad_name_pods sts pods : list PodV.t :=
-  filter (λ pod, ¬ pod_has_member_key sts pod) pods.
-
-Definition condemned_pods sts pods : list PodV.t :=
-  filter (λ pod, pod_has_member_key sts pod ∧ ¬ pod_key_is_desired sts (PodV.key pod)) pods.
-
-(* The progress metric gives an outdated desired Pod cost 2 and a missing
-   desired Pod cost 1, so deleting one outdated Pod strictly reduces the
-   distance even though the desired replacement Pod is created by a later run.
-   Once the delete only sets DeletionTimestamp, the Pod is no longer alive and
-   should not keep contributing to the outdated-Pod distance. *)
-Definition pod_distance sts pods : nat :=
-  length (missing_pod_keys sts pods) +
-  2 * length (filter is_pod_alive (outdated_pods sts pods)) +
-  length (filter is_pod_alive (condemned_pods sts pods)) +
-  length (bad_name_pods sts pods).
-
-Definition missing_pvc_keys sts (pvcs : list PersistentVolumeClaimV.t) : list KKey.t :=
-  filter (λ key, key ∉ (PersistentVolumeClaimV.key <$> pvcs)) (desired_pvc_keys sts).
-
-Definition pvc_distance sts pvcs : nat :=
-  length (missing_pvc_keys sts pvcs).
-
-Definition match_distance sts pods pvcs : nat :=
-  pod_distance sts pods + pvc_distance sts pvcs.
-
-Definition pods_match sts pods : Prop :=
-  PodV.key <$> pods ≡ₚ desired_pod_keys sts ∧
-  Forall is_pod_alive pods ∧
-  Forall (pod_match sts) pods.
-
-Definition pvcs_match sts (pvcs : list PersistentVolumeClaimV.t) : Prop :=
-  ∀ key, key ∈ desired_pvc_keys sts →
-    key ∈ (PersistentVolumeClaimV.key <$> pvcs).
-
-Definition current_state_matches sts pods pvcs : Prop :=
-  pods_match sts pods ∧ pvcs_match sts pvcs.
-
-Lemma match_distance_zero_matches γ sts pods pvcs :
-  (∀ pod, pod ∈ pods → is_pod_alive pod) →
-  ([∗ list] pod ∈ pods, own_meta_frag γ (PodV.key pod) pod.(PodV.ObjectMeta').(ObjectMetaV.UID') 1 pod.(PodV.ObjectMeta')) -∗
-  ⌜ match_distance sts pods pvcs = 0%nat ↔ current_state_matches sts pods pvcs ⌝.
-Proof.
-  iIntros (Hpods_alive) "Hpod_meta_frags".
-  iPoseProof (kview.own_meta_list_no_dup PodV.key PodV.ObjectMeta'
-    with "Hpod_meta_frags") as "%Hpods_nodup".
-  iPureIntro.
-  assert (Hdesired_pods_nodup : NoDup (desired_pod_keys sts)).
-  { unfold desired_pod_keys, desired_ordinals.
-    apply NoDup_fmap_2.
-    - intros ordinal1 ordinal2 Hkey.
-      apply (f_equal KKey.Name') in Hkey.
-      simpl in Hkey.
-      unfold desired_pod_name in Hkey.
-      simpl in Hkey.
-      apply app_inv_head in Hkey.
-      inversion Hkey as [Hdecimal].
-      by apply decimal_string_inj in Hdecimal.
-    - apply NoDup_seq. }
-	split.
-	- intros Hdist.
-	  unfold match_distance, pod_distance, pvc_distance in Hdist.
-	  assert (Hmissing_pods : length (missing_pod_keys sts pods) = 0%nat) by lia.
-    assert (Halive_outdated_pods :
-        length (filter is_pod_alive (outdated_pods sts pods)) = 0%nat) by lia.
-    assert (Hbad_name_pods : length (bad_name_pods sts pods) = 0%nat) by lia.
-    assert (Halive_condemned_pods :
-        length (filter is_pod_alive (condemned_pods sts pods)) = 0%nat) by lia.
-    assert (Hmissing_pvcs : length (missing_pvc_keys sts pvcs) = 0%nat) by lia.
-    assert (Hpod_good_name : ∀ pod,
-        pod ∈ pods → pod_has_member_key sts pod).
-    { intros pod Hpod.
-      destruct (decide (pod_has_member_key sts pod)) as [Hgood|Hbad]; [done|].
-      exfalso.
-      eapply (filter_length_zero_not_elem
-        (λ pod, ¬ pod_has_member_key sts pod) pods pod);
-        [exact Hbad_name_pods|exact Hpod|exact Hbad]. }
-    assert (Hdesired_pod_actual : ∀ key,
-        key ∈ desired_pod_keys sts → key ∈ PodV.key <$> pods).
-	  { intros key Hdesired.
-	    destruct (decide (key ∈ PodV.key <$> pods)) as [Hactual|Hnot_actual]; [done|].
-	    exfalso.
-	    eapply (filter_length_zero_not_elem
-	      (λ key, key ∉ (PodV.key <$> pods)) (desired_pod_keys sts) key);
-	      [exact Hmissing_pods|exact Hdesired|exact Hnot_actual]. }
-	  assert (Hactual_pod_desired : ∀ pod,
-	      pod ∈ pods → pod_key_is_desired sts (PodV.key pod)).
-	  { intros pod Hpod.
-	    destruct (decide (pod_key_is_desired sts (PodV.key pod))) as [Hdesired|Hnot_desired]; [done|].
-	    exfalso.
-	    assert (Hpod_condemned : pod ∈ condemned_pods sts pods).
-	    { unfold condemned_pods.
-	      apply list_elem_of_filter. split; [split; [by apply Hpod_good_name|exact Hnot_desired]|exact Hpod]. }
-	    eapply (filter_length_zero_not_elem
-	      is_pod_alive (condemned_pods sts pods) pod);
-	      [exact Halive_condemned_pods|exact Hpod_condemned|by apply Hpods_alive]. }
-	  assert (Hpods_perm : PodV.key <$> pods ≡ₚ desired_pod_keys sts).
-	  { apply NoDup_Permutation; [exact Hpods_nodup|exact Hdesired_pods_nodup|].
-	    intros key. split.
-	    - intros Hactual.
-	      apply list_elem_of_fmap_1 in Hactual as (pod & Hkey_eq & Hpod).
-	      rewrite Hkey_eq. by apply Hactual_pod_desired.
-	    - intros Hdesired. by apply Hdesired_pod_actual. }
-	  split.
-	  + split; [exact Hpods_perm|].
-	    split.
-	    * apply Forall_forall. intros pod Hpod.
-	      rewrite <- list_elem_of_In in Hpod.
-	      by apply Hpods_alive.
-	    * apply Forall_forall. intros pod Hpod.
-	      rewrite <- list_elem_of_In in Hpod.
-	      destruct (decide (pod_match sts pod)) as [Hmatch|Hnot_match]; [exact Hmatch|].
-	      exfalso.
-	      assert (Hpod_needed : pod ∈ needed_pods sts pods).
-	      { unfold needed_pods.
-	        apply list_elem_of_filter. split; [by apply Hactual_pod_desired|exact Hpod]. }
-	      assert (Hpod_outdated : pod ∈ outdated_pods sts pods).
-	      { unfold outdated_pods.
-	        apply list_elem_of_filter. split; [exact Hnot_match|exact Hpod_needed]. }
-	      eapply (filter_length_zero_not_elem
-	        is_pod_alive
-	        (outdated_pods sts pods) pod);
-	        [exact Halive_outdated_pods|exact Hpod_outdated|].
-	      by apply Hpods_alive.
-	  + intros key Hdesired.
-	    destruct (decide (key ∈ PersistentVolumeClaimV.key <$> pvcs)) as [Hactual|Hnot_actual]; [done|].
-	    exfalso.
-	    eapply (filter_length_zero_not_elem
-	      (λ key, key ∉ (PersistentVolumeClaimV.key <$> pvcs)) (desired_pvc_keys sts) key);
-	      [exact Hmissing_pvcs|exact Hdesired|exact Hnot_actual].
-	- intros [[Hpods_perm [Hpods_alive_forall Hpods_match_forall]] Hpvcs_match].
-	  unfold match_distance, pod_distance, pvc_distance.
-	  assert (Hmissing_pods_nil : missing_pod_keys sts pods = []).
-	  { unfold missing_pod_keys.
-	    apply filter_none. intros key Hdesired Hnot_actual.
-	    apply Hnot_actual.
-	    rewrite Hpods_perm. exact Hdesired. }
-	  assert (Houtdated_pods_nil : outdated_pods sts pods = []).
-	  { unfold outdated_pods.
-	    apply filter_none. intros pod Hpod Hnot_match.
-	    rewrite Forall_forall in Hpods_match_forall.
-	    unfold needed_pods in Hpod.
-	    apply list_elem_of_filter in Hpod as [_ Hpod].
-	    rewrite list_elem_of_In in Hpod.
-	    exact (Hnot_match (Hpods_match_forall pod Hpod)). }
-	  assert (Hbad_name_pods_nil : bad_name_pods sts pods = []).
-	  { unfold bad_name_pods.
-	    apply filter_none. intros pod Hpod Hnot_member.
-	    apply Hnot_member.
-	    assert (Hkey_desired : PodV.key pod ∈ desired_pod_keys sts).
-	    { rewrite -Hpods_perm. by apply list_elem_of_fmap_2. }
-	    unfold desired_pod_keys in Hkey_desired.
-	    apply list_elem_of_fmap_1 in Hkey_desired as (ordinal & Hkey_eq & _).
-	    exists ordinal. exact Hkey_eq. }
-	  assert (Halive_condemned_pods_nil : filter is_pod_alive (condemned_pods sts pods) = []).
-	  { apply filter_none. intros pod Hpod Halive.
-	    unfold condemned_pods in Hpod.
-	    apply list_elem_of_filter in Hpod as ((_ & Hnot_desired) & Hpod).
-	    apply Hnot_desired.
-	    unfold pod_key_is_desired.
-	    rewrite -Hpods_perm. by apply list_elem_of_fmap_2. }
-	  assert (Hmissing_pvcs_nil : missing_pvc_keys sts pvcs = []).
-	  { unfold missing_pvc_keys.
-	    apply filter_none. intros key Hdesired Hnot_actual.
-      apply Hnot_actual. by apply Hpvcs_match. }
-    rewrite Hmissing_pods_nil Houtdated_pods_nil Hbad_name_pods_nil
-      Halive_condemned_pods_nil Hmissing_pvcs_nil.
-    done.
-Qed.
-
-Definition pod_meta_except_resource_version_changed
-    (pods pods' : list PodV.t) : Prop :=
-  ∃ pod pod',
-    pod ∈ pods ∧
-    pod' ∈ pods' ∧
-    PodV.key pod = PodV.key pod' ∧
-    ObjectMetaV.without_resource_version pod.(PodV.ObjectMeta') ≠
-      ObjectMetaV.without_resource_version pod'.(PodV.ObjectMeta').
-
-Definition pod_spec_changed (pods pods' : list PodV.t) : Prop :=
-  ∃ pod pod',
-    pod ∈ pods ∧
-    pod' ∈ pods' ∧
-    PodV.key pod = PodV.key pod' ∧
-    pod.(PodV.Spec') ≠ pod'.(PodV.Spec').
-
-Definition pods_progress_observed (pods pods' : list PodV.t) : Prop :=
-  list_to_set (C:=gset KKey.t) (PodV.key <$> pods) ≠
-    list_to_set (C:=gset KKey.t) (PodV.key <$> pods') ∨
-  pod_meta_except_resource_version_changed pods pods' ∨
-  pod_spec_changed pods pods'.
+Definition input_requirement (sts : StatefulSetV.t) : Prop :=
+  (* StatefulSet admission validates the set name before the controller adds
+     the ordinal suffix. Require every generated Pod name to remain a valid
+     DNS-1123 label because it is also used as the Pod hostname and as a label
+     value, both of which have a 63-byte limit. *)
+  (∀ ordinal,
+    (ordinal < statefulset_replicas sts)%nat →
+    valid_dns1123_label
+      (desired_pod_name
+        sts.(StatefulSetV.ObjectMeta').(ObjectMetaV.Name') ordinal)) ∧
+  (* StatefulSet admission does not validate Pod-template finalizers, but the
+     controller copies them to generated Pods and Pod create validates them. *)
+  valid_finalizers
+    ((sts.(StatefulSetV.Spec').(StatefulSetSpecV.Template')).(PodTemplateSpecV.ObjectMeta').(ObjectMetaV.Finalizers')) ∧
+  (* StatefulSet admission validates only each volume-claim template's spec.
+     The controller copies its otherwise-unvalidated metadata to generated
+     PVCs, whose full metadata is validated on create. *)
+  Forall
+    (λ claim_template,
+      ∀ ordinal,
+        (ordinal < statefulset_replicas sts)%nat →
+        PersistentVolumeClaimV.valid_named_create
+          sts.(StatefulSetV.ObjectMeta').(ObjectMetaV.Namespace')
+          (new_persistent_volume_claim sts claim_template ordinal))
+    sts.(StatefulSetV.Spec').(StatefulSetSpecV.VolumeClaimTemplates').
 
 Lemma wp_syncStatefulSet_progress γ l namespace name sts dq pods pvcs :
   {{{ is_pkg_init code.controllers.statefulset.pkg_id.statefulset ∗
@@ -255,20 +80,16 @@ Lemma wp_syncStatefulSet_progress γ l namespace name sts dq pods pvcs :
       "Hown_children_frag" ∷ own_children_frag γ (StatefulSetV.key sts) sts.(StatefulSetV.ObjectMeta').(ObjectMetaV.UID') 1 (list_to_set (PodV.key <$> pods)) ∗
       "Hown_reserved_missing_pod_keys" ∷ ([∗ list] key ∈ missing_pod_keys sts pods, own_reserved_frag γ key) ∗
       "Hown_reserved_missing_pvc_keys" ∷ ([∗ list] key ∈ missing_pvc_keys sts pvcs, own_reserved_frag γ key) ∗
+      "%Hpending_pods_empty" ∷ ⌜ filter (pending_pod sts) pods = [] ⌝ ∗
+      "%Hinput_requirement" ∷ ⌜ input_requirement sts ⌝ ∗
       "%Hnamespace_eq" ∷ ⌜ namespace = sts.(StatefulSetV.ObjectMeta').(ObjectMetaV.Namespace') ⌝ ∗
       "%Hname_eq" ∷ ⌜ name = sts.(StatefulSetV.ObjectMeta').(ObjectMetaV.Name') ⌝ ∗
       "%Hdeletion_timestamp_eq" ∷ ⌜ sts.(StatefulSetV.ObjectMeta').(ObjectMetaV.DeletionTimestamp') = None ⌝
   }}}
     @! statefulset.syncStatefulSet #namespace #name
   {{{ (pods' : list PodV.t) (pvcs' : list PersistentVolumeClaimV.t) (err : interface.t), RET #err;
-      (* We expect one of the three cases when reconcile finishes:
-        (1) the current state (pods' and pvcs') matches the desired state encoded in sts,
-        (2) the distance is reduced and a new reoncile is rescheduled because of changes to pods
-        (3) the distance doesn't get increased because the controller needs to wait for some terminating pods
-      *)
       ⌜ current_state_matches sts pods' pvcs' ∨
-        pods_progress_observed pods pods' ∧ match_distance sts pods' pvcs' < match_distance sts pods pvcs ∨
-        (∃ pod, pod ∈ pods ∧ ¬ is_pod_alive pod) ∧ match_distance sts pods' pvcs' ≤ match_distance sts pods pvcs ⌝ ∗
+        pods_progress_observed pods pods' ∧ match_distance sts pods' pvcs' < match_distance sts pods pvcs ⌝ ∗
       own_meta_frag γ (StatefulSetV.key sts) sts.(StatefulSetV.ObjectMeta').(ObjectMetaV.UID') dq sts.(StatefulSetV.ObjectMeta') ∗
       own_spec_frag γ (StatefulSetV.key sts) sts.(StatefulSetV.ObjectMeta').(ObjectMetaV.UID') dq (ObjectSpecV.StatefulSetSpec sts.(StatefulSetV.Spec')) ∗
       ([∗ list] pod ∈ pods',
