src/proof/controllers/statefulset/distance.v
@@ -1,0 +1,243 @@
+From New.proof.controllers.statefulset Require Export pod.
+
+Section proof.
+Context `{hG: !heapGS Σ} `{!ffi_semantics _ _}.
+Context {sem : go.Semantics}
+  {package_sem : code.controllers.statefulset.statefulset.Assumptions}.
+Collection W := sem + package_sem.
+#[local] Instance base_common_sem : common.Assumptions | 100 :=
+  code.controllers.statefulset.statefulset.import_common_Assumption.
+#[local] Instance controller_sem : controller.Assumptions :=
+  code.controllers.statefulset.statefulset.import_controller_Assumption.
+#[local] Instance runtime_sem : code.k8s_io.apimachinery.pkg.runtime.runtime.Assumptions :=
+  controller.import_runtime_Assumption.
+#[local] Instance runtime_object_underlying_eq :
+    runtime.Object ≤u runtime.Objectⁱᵐᵖˡ.
+Proof using package_sem. apply _. Qed.
+#[local] Instance meta_object_underlying_eq :
+    meta_v1.Object ≤u meta_v1.Objectⁱᵐᵖˡ.
+Proof using package_sem. apply _. Qed.
+#[local] Instance base_apimodel_sem : apimodel.Assumptions | 100 :=
+  common.import_apimodel_Assumption.
+#[local] Instance object_meta_v1_sem :
+    code.k8s_io.apimachinery.pkg.apis.meta.v1.v1.Assumptions :=
+  apimodel.import_apis_meta_v1_Assumption.
+#[local] Instance object_apps_v1_sem :
+    code.k8s_io.api.apps.v1.v1.Assumptions :=
+  apimodel.import_api_apps_v1_Assumption.
+#[local] Instance object_core_v1_sem :
+    code.k8s_io.api.core.v1.v1.Assumptions :=
+  code.k8s_io.api.apps.v1.v1.import_core_v1_Assumption.
+#[local] Instance apimodel_sem : apimodel.Assumptions | 0.
+Proof using package_sem.
+  constructor; try exact object_core_v1_sem; try apply _.
+Defined.
+#[local] Instance common_sem : common.Assumptions | 0.
+Proof using package_sem.
+  constructor; try exact apimodel_sem; try apply _.
+Defined.
+Context `{!kubernetesModelG Σ}.
+Local Set Default Proof Using "All".
+
+Definition missing_pod_keys sts (pods : list PodV.t) : list KKey.t :=
+  filter (λ key, key ∉ (PodV.key <$> pods)) (desired_pod_keys sts).
+
+Definition needed_pods sts pods : list PodV.t :=
+  filter (λ pod, pod_key_is_desired sts (PodV.key pod)) pods.
+
+Definition outdated_pods sts pods : list PodV.t :=
+  filter (λ pod, ¬ pod_match sts pod) (needed_pods sts pods).
+
+Definition bad_name_pods sts pods : list PodV.t :=
+  filter (λ pod, ¬ pod_has_member_key sts pod) pods.
+
+Definition condemned_pods sts pods : list PodV.t :=
+  filter (λ pod, pod_has_member_key sts pod ∧ ¬ pod_key_is_desired sts (PodV.key pod)) pods.
+
+(* The progress metric gives an outdated desired Pod cost 2 and a missing
+   desired Pod cost 1, so deleting one outdated Pod strictly reduces the
+   distance even though the desired replacement Pod is created by a later run.
+   Once the delete only sets DeletionTimestamp, the Pod is no longer alive and
+   should not keep contributing to the outdated-Pod distance. *)
+Definition pod_distance sts pods : nat :=
+  length (missing_pod_keys sts pods) +
+  2 * length (filter is_pod_alive (outdated_pods sts pods)) +
+  length (filter is_pod_alive (condemned_pods sts pods)) +
+  length (bad_name_pods sts pods).
+
+Definition missing_pvc_keys sts (pvcs : list PersistentVolumeClaimV.t) : list KKey.t :=
+  filter (λ key, key ∉ (PersistentVolumeClaimV.key <$> pvcs)) (desired_pvc_keys sts).
+
+Definition pvc_distance sts pvcs : nat :=
+  length (missing_pvc_keys sts pvcs).
+
+Definition match_distance sts pods pvcs : nat :=
+  pod_distance sts pods + pvc_distance sts pvcs.
+
+Definition pods_match sts pods : Prop :=
+  PodV.key <$> pods ≡ₚ desired_pod_keys sts ∧
+  Forall is_pod_alive pods ∧
+  Forall (pod_match sts) pods.
+
+Definition pvcs_match sts (pvcs : list PersistentVolumeClaimV.t) : Prop :=
+  ∀ key, key ∈ desired_pvc_keys sts →
+    key ∈ (PersistentVolumeClaimV.key <$> pvcs).
+
+Definition current_state_matches sts pods pvcs : Prop :=
+  pods_match sts pods ∧ pvcs_match sts pvcs.
+
+Lemma match_distance_zero_matches γ sts pods pvcs :
+  (∀ pod, pod ∈ pods → is_pod_alive pod) →
+  ([∗ list] pod ∈ pods, own_meta_frag γ (PodV.key pod) pod.(PodV.ObjectMeta').(ObjectMetaV.UID') 1 pod.(PodV.ObjectMeta')) -∗
+  ⌜ match_distance sts pods pvcs = 0%nat ↔ current_state_matches sts pods pvcs ⌝.
+Proof.
+  iIntros (Hpods_alive) "Hpod_meta_frags".
+  iPoseProof (kview.own_meta_list_no_dup PodV.key PodV.ObjectMeta'
+    with "Hpod_meta_frags") as "%Hpods_nodup".
+  iPureIntro.
+  assert (Hdesired_pods_nodup : NoDup (desired_pod_keys sts)).
+  { unfold desired_pod_keys, desired_ordinals.
+    apply NoDup_fmap_2.
+    - intros ordinal1 ordinal2 Hkey.
+      apply (f_equal KKey.Name') in Hkey.
+      simpl in Hkey.
+      unfold desired_pod_name in Hkey.
+      simpl in Hkey.
+      apply app_inv_head in Hkey.
+      inversion Hkey as [Hdecimal].
+      by apply decimal_string_inj in Hdecimal.
+    - apply NoDup_seq. }
+  split.
+  - intros Hdist.
+    unfold match_distance, pod_distance, pvc_distance in Hdist.
+    assert (Hmissing_pods : length (missing_pod_keys sts pods) = 0%nat) by lia.
+    assert (Halive_outdated_pods :
+        length (filter is_pod_alive (outdated_pods sts pods)) = 0%nat) by lia.
+    assert (Hbad_name_pods : length (bad_name_pods sts pods) = 0%nat) by lia.
+    assert (Halive_condemned_pods :
+        length (filter is_pod_alive (condemned_pods sts pods)) = 0%nat) by lia.
+    assert (Hmissing_pvcs : length (missing_pvc_keys sts pvcs) = 0%nat) by lia.
+    assert (Hpod_good_name : ∀ pod,
+        pod ∈ pods → pod_has_member_key sts pod).
+    { intros pod Hpod.
+      destruct (decide (pod_has_member_key sts pod)) as [Hgood|Hbad]; [done|].
+      exfalso.
+      eapply (filter_length_zero_not_elem
+        (λ pod, ¬ pod_has_member_key sts pod) pods pod);
+        [exact Hbad_name_pods|exact Hpod|exact Hbad]. }
+    assert (Hdesired_pod_actual : ∀ key,
+        key ∈ desired_pod_keys sts → key ∈ PodV.key <$> pods).
+    { intros key Hdesired.
+      destruct (decide (key ∈ PodV.key <$> pods)) as [Hactual|Hnot_actual]; [done|].
+      exfalso.
+      eapply (filter_length_zero_not_elem
+        (λ key, key ∉ (PodV.key <$> pods)) (desired_pod_keys sts) key);
+        [exact Hmissing_pods|exact Hdesired|exact Hnot_actual]. }
+    assert (Hactual_pod_desired : ∀ pod,
+        pod ∈ pods → pod_key_is_desired sts (PodV.key pod)).
+    { intros pod Hpod.
+      destruct (decide (pod_key_is_desired sts (PodV.key pod))) as [Hdesired|Hnot_desired]; [done|].
+      exfalso.
+      assert (Hpod_condemned : pod ∈ condemned_pods sts pods).
+      { unfold condemned_pods.
+        apply list_elem_of_filter. split; [split; [by apply Hpod_good_name|exact Hnot_desired]|exact Hpod]. }
+      eapply (filter_length_zero_not_elem
+        is_pod_alive (condemned_pods sts pods) pod);
+        [exact Halive_condemned_pods|exact Hpod_condemned|by apply Hpods_alive]. }
+    assert (Hpods_perm : PodV.key <$> pods ≡ₚ desired_pod_keys sts).
+    { apply NoDup_Permutation; [exact Hpods_nodup|exact Hdesired_pods_nodup|].
+      intros key. split.
+      - intros Hactual.
+        apply list_elem_of_fmap_1 in Hactual as (pod & Hkey_eq & Hpod).
+        rewrite Hkey_eq. by apply Hactual_pod_desired.
+      - intros Hdesired. by apply Hdesired_pod_actual. }
+    split.
+    + split; [exact Hpods_perm|].
+      split.
+      * apply Forall_forall. intros pod Hpod.
+        rewrite <- list_elem_of_In in Hpod.
+        by apply Hpods_alive.
+      * apply Forall_forall. intros pod Hpod.
+        rewrite <- list_elem_of_In in Hpod.
+        destruct (decide (pod_match sts pod)) as [Hmatch|Hnot_match]; [exact Hmatch|].
+        exfalso.
+        assert (Hpod_needed : pod ∈ needed_pods sts pods).
+        { unfold needed_pods.
+          apply list_elem_of_filter. split; [by apply Hactual_pod_desired|exact Hpod]. }
+        assert (Hpod_outdated : pod ∈ outdated_pods sts pods).
+        { unfold outdated_pods.
+          apply list_elem_of_filter. split; [exact Hnot_match|exact Hpod_needed]. }
+        eapply (filter_length_zero_not_elem
+          is_pod_alive
+          (outdated_pods sts pods) pod);
+          [exact Halive_outdated_pods|exact Hpod_outdated|].
+        by apply Hpods_alive.
+    + intros key Hdesired.
+      destruct (decide (key ∈ PersistentVolumeClaimV.key <$> pvcs)) as [Hactual|Hnot_actual]; [done|].
+      exfalso.
+      eapply (filter_length_zero_not_elem
+        (λ key, key ∉ (PersistentVolumeClaimV.key <$> pvcs)) (desired_pvc_keys sts) key);
+        [exact Hmissing_pvcs|exact Hdesired|exact Hnot_actual].
+  - intros [[Hpods_perm [Hpods_alive_forall Hpods_match_forall]] Hpvcs_match].
+    unfold match_distance, pod_distance, pvc_distance.
+    assert (Hmissing_pods_nil : missing_pod_keys sts pods = []).
+    { unfold missing_pod_keys.
+      apply filter_none. intros key Hdesired Hnot_actual.
+      apply Hnot_actual.
+      rewrite Hpods_perm. exact Hdesired. }
+    assert (Houtdated_pods_nil : outdated_pods sts pods = []).
+    { unfold outdated_pods.
+      apply filter_none. intros pod Hpod Hnot_match.
+      rewrite Forall_forall in Hpods_match_forall.
+      unfold needed_pods in Hpod.
+      apply list_elem_of_filter in Hpod as [_ Hpod].
+      rewrite list_elem_of_In in Hpod.
+      exact (Hnot_match (Hpods_match_forall pod Hpod)). }
+    assert (Hbad_name_pods_nil : bad_name_pods sts pods = []).
+    { unfold bad_name_pods.
+      apply filter_none. intros pod Hpod Hnot_member.
+      apply Hnot_member.
+      assert (Hkey_desired : PodV.key pod ∈ desired_pod_keys sts).
+      { rewrite -Hpods_perm. by apply list_elem_of_fmap_2. }
+      unfold desired_pod_keys in Hkey_desired.
+      apply list_elem_of_fmap_1 in Hkey_desired as (ordinal & Hkey_eq & _).
+      exists ordinal. exact Hkey_eq. }
+    assert (Halive_condemned_pods_nil : filter is_pod_alive (condemned_pods sts pods) = []).
+    { apply filter_none. intros pod Hpod Halive.
+      unfold condemned_pods in Hpod.
+      apply list_elem_of_filter in Hpod as ((_ & Hnot_desired) & Hpod).
+      apply Hnot_desired.
+      unfold pod_key_is_desired.
+      rewrite -Hpods_perm. by apply list_elem_of_fmap_2. }
+    assert (Hmissing_pvcs_nil : missing_pvc_keys sts pvcs = []).
+    { unfold missing_pvc_keys.
+      apply filter_none. intros key Hdesired Hnot_actual.
+      apply Hnot_actual. by apply Hpvcs_match. }
+    rewrite Hmissing_pods_nil Houtdated_pods_nil Hbad_name_pods_nil
+      Halive_condemned_pods_nil Hmissing_pvcs_nil.
+    done.
+Qed.
+
+Definition pod_meta_except_resource_version_changed
+    (pods pods' : list PodV.t) : Prop :=
+  ∃ pod pod',
+    pod ∈ pods ∧
+    pod' ∈ pods' ∧
+    PodV.key pod = PodV.key pod' ∧
+    ObjectMetaV.without_resource_version pod.(PodV.ObjectMeta') ≠
+      ObjectMetaV.without_resource_version pod'.(PodV.ObjectMeta').
+
+Definition pod_spec_changed (pods pods' : list PodV.t) : Prop :=
+  ∃ pod pod',
+    pod ∈ pods ∧
+    pod' ∈ pods' ∧
+    PodV.key pod = PodV.key pod' ∧
+    pod.(PodV.Spec') ≠ pod'.(PodV.Spec').
+
+Definition pods_progress_observed (pods pods' : list PodV.t) : Prop :=
+  list_to_set (C:=gset KKey.t) (PodV.key <$> pods) ≠
+    list_to_set (C:=gset KKey.t) (PodV.key <$> pods') ∨
+  pod_meta_except_resource_version_changed pods pods' ∨
+  pod_spec_changed pods pods'.
+
+End proof.
